proof/invariant-abstract/RISCV64/ArchInvariants_AI.thy
@@ -571,12 +571,12 @@ definition vspace_at_asid :: "asid \<Rightarrow> obj_ref \<Rightarrow> 'z::state
 definition valid_uses_2 :: "(obj_ref \<Rightarrow> riscvvspace_region_use) \<Rightarrow> bool" where
   "valid_uses_2 uses \<equiv>
      \<forall>p. (\<not>canonical_address p \<longrightarrow> uses p = RISCVVSpaceInvalidRegion)
-          \<and> (p \<in> {pptr_base ..< kernel_base}
+          \<and> (p \<in> {pptr_base ..< kernel_elf_base}
              \<longrightarrow> uses p \<in> {RISCVVSpaceKernelWindow, RISCVVSpaceInvalidRegion})
-          \<and> (uses p = RISCVVSpaceKernelWindow \<longrightarrow> p \<in> {pptr_base ..< kernel_base})
+          \<and> (uses p = RISCVVSpaceKernelWindow \<longrightarrow> p \<in> {pptr_base ..< kernel_elf_base})
           \<comment> \<open>Ordinarily there would be another region on top of the RISCVVSpaceKernelELFWindow
              for devices, but Spike does not have any.\<close>
-          \<and> (kernel_base \<le> p \<longrightarrow> uses p \<in> {RISCVVSpaceKernelELFWindow, RISCVVSpaceInvalidRegion})
+          \<and> (kernel_elf_base \<le> p \<longrightarrow> uses p \<in> {RISCVVSpaceKernelELFWindow, RISCVVSpaceInvalidRegion})
           \<comment> \<open>We allow precisely all virtual addresses up to canonical_user as the user window:\<close>
           \<and> (user_region = user_window_2 uses)
       \<comment> \<open>We want the kernel window to be non-empty, and to contain at least @{const pptr_base}\<close>
@@ -1289,9 +1289,9 @@ lemma canonical_user_pptr_base:
   "canonical_user < pptr_base"
   by (simp add: canonical_user_def pptr_base_def pptrBase_def canonical_bit_def mask_def)
 
-lemma pptr_base_kernel_base:
-  "pptr_base < kernel_base"
-  by (simp add: pptr_base_def pptrBase_def canonical_bit_def kernel_base_def)
+lemma pptr_base_kernel_elf_base:
+  "pptr_base < kernel_elf_base"
+  by (simp add: pptr_base_def pptrBase_def canonical_bit_def kernel_elf_base_def)
 
 lemma above_pptr_base_canonical:
   "pptr_base \<le> p \<Longrightarrow> canonical_address p"
@@ -1314,7 +1314,7 @@ lemmas window_defs =
   kernel_device_window_def user_region_def user_window_def
 
 lemma valid_uses_kernel_window:
-  "\<lbrakk> valid_uses s; p \<in> kernel_window s \<rbrakk> \<Longrightarrow> p \<in> {pptr_base ..< kernel_base} \<and> canonical_address p"
+  "\<lbrakk> valid_uses s; p \<in> kernel_window s \<rbrakk> \<Longrightarrow> p \<in> {pptr_base ..< kernel_elf_base} \<and> canonical_address p"
   unfolding valid_uses_def window_defs
   by (erule_tac x=p in allE) auto
 
